state-syncer/src/bin/hint_gen/fast_path.rs
@@ -1,0 +1,58 @@
+use state_syncer::iprf::Iprf;
+
+use crate::hint_gen::subsets::{block_in_subset, xor_32};
+use crate::hint_gen::types::{BackupHint, RegularHint, WORD_SIZE};
+
+pub fn process_entries_fast(
+    db_bytes: &[u8],
+    n_entries: usize,
+    n_effective: usize,
+    w: usize,
+    _c: usize,
+    num_regular: usize,
+    num_backup: usize,
+    block_iprfs: &[Iprf],
+    regular_hint_blocks: &[Vec<usize>],
+    backup_hint_blocks: &[Vec<usize>],
+    regular_hints: &mut [RegularHint],
+    backup_hints: &mut [BackupHint],
+    progress_callback: impl Fn(usize),
+) {
+    for i in 0..n_effective {
+        let block = i / w;
+        let offset = i % w;
+
+        let entry: [u8; 32] = if i < n_entries {
+            let entry_offset = i * WORD_SIZE;
+            db_bytes[entry_offset..entry_offset + WORD_SIZE]
+                .try_into()
+                .unwrap()
+        } else {
+            [0u8; 32]
+        };
+
+        let hint_indices = block_iprfs[block].inverse(offset as u64);
+
+        for j in hint_indices {
+            let j = j as usize;
+            if j < num_regular {
+                if block_in_subset(&regular_hint_blocks[j], block) {
+                    xor_32(&mut regular_hints[j].parity, &entry);
+                }
+            } else {
+                let backup_idx = j - num_regular;
+                if backup_idx < num_backup {
+                    if block_in_subset(&backup_hint_blocks[backup_idx], block) {
+                        xor_32(&mut backup_hints[backup_idx].parity_in, &entry);
+                    } else {
+                        xor_32(&mut backup_hints[backup_idx].parity_out, &entry);
+                    }
+                }
+            }
+        }
+
+        if i % 10000 == 0 {
+            progress_callback(i);
+        }
+    }
+}
